fix(repr): Interval interaction across octave

Prismriver/Repr/Classical.lean
@@ -102,6 +102,7 @@ protected def Hep.toNat (h : Hep) := (h : Fin 7).toNat
 /-- Semitone spaces between names -/
 def spaces := [2, 2, 1, 2, 2, 2, 1]
 
+/-- Equivalence classes of pitches modulo octave -/
 structure Tone where
   name : Hep
   acc : Accidental := .natural
@@ -254,45 +255,49 @@ def minorTriad (p : Pitch) : List Pitch := [
 end Interval
 
 /-- Interval with only a name distance in a particular key. Also known as a generic interval -/
-structure KeyInterval (modus : Hep) where
+structure KeyInterval (root modus : Hep) where
   name : Int
 
-instance : HAdd Pitch (KeyInterval modus) Pitch where
+instance : HAdd Pitch (KeyInterval root modus) Pitch where
   hAdd p i :=
     let name := p.name + i.name
-    -- If the modus is C, there should not be any shift
+    -- If the modus and root are equal, there should not be any shift since there are no flats or sharps
     let distance := i.name.fmod 7 |>.toNat
-    let shiftModus : Int := (p.name.toNat + modus.toNat).repeat List.rotateRight spaces
+    let s1 := p.name.toNat + modus.toNat + 7 - root.toNat
+    let shiftModus : Int := s1.repeat List.rotateLeft spaces
       |>.take distance |>.sum
-    let shiftNominal : Int := p.name.toNat.repeat List.rotateRight spaces
+    let shiftNominal : Int := (p.name.toNat).repeat List.rotateLeft spaces
       |>.take distance |>.sum
-    --let Δsemitones := shiftNominal - shiftModus
-    let Δsemitones := shiftNominal - shiftModus
+    let Δsemitones := shiftModus - shiftNominal
     { name, acc := { semitones := p.acc.semitones + Δsemitones } }
-instance : Neg (KeyInterval root) where
+instance : Neg (KeyInterval root modus) where
   neg i := { name := -i.name }
 
-example : (Pitch.new .a 3) + (⟨1⟩ : KeyInterval .d) = (Pitch.new .b 3 .flat) := rfl
-example : (Pitch.new .a 3) + (⟨8⟩ : KeyInterval .d) = (Pitch.new .b 4 .flat) := rfl
-example : (Pitch.new .a 3) + (⟨9⟩ : KeyInterval .d) = (Pitch.new .c 5) := rfl
-example : (Pitch.new .c 4) + (⟨2⟩ : KeyInterval .c) = (Pitch.new .e 4) := rfl
+example : (Pitch.new .c 4) + (⟨2⟩ : KeyInterval .c .c) = (Pitch.new .e 4) := rfl
+example : (Pitch.new .c 4) + (⟨3⟩ : KeyInterval .c .c) = (Pitch.new .f 4) := rfl
+example : (Pitch.new .c 4) + (⟨-1⟩ : KeyInterval .c .c) = (Pitch.new .b 3) := rfl
+example : (Pitch.new .a 3) + (⟨1⟩ : KeyInterval .d .a) = (Pitch.new .b 3 .flat) := rfl
+example : (Pitch.new .a 3) + (⟨8⟩ : KeyInterval .d .a) = (Pitch.new .b 4 .flat) := rfl
+example : (Pitch.new .a 3) + (⟨9⟩ : KeyInterval .d .a) = (Pitch.new .c 5) := rfl
+example : (Pitch.new .d 4) + (⟨5⟩ : KeyInterval .d .a) = (Pitch.new .b 4 .flat) := rfl
+example : (Pitch.new .d 4) + (⟨4⟩ : KeyInterval .d .d) = (Pitch.new .a 4) := rfl
 
-instance : Add (KeyInterval modus) where
+instance : Add (KeyInterval root modus) where
   add x y := { name := x.name + y.name }
-instance : Sub (KeyInterval modus) where
+instance : Sub (KeyInterval root modus) where
   sub x y := { name := x.name - y.name }
-instance : SMul Int (KeyInterval modus) where
+instance : SMul Int (KeyInterval root modus) where
   smul n x := { name := n * x.name }
-instance : Neg (KeyInterval modus) where
+instance : Neg (KeyInterval root modus) where
   neg i := { name := -i.name }
 
 namespace KeyInterval
 
-protected def zero { modus : Hep } : KeyInterval modus := ⟨0⟩
+protected def zero { root modus : Hep } : KeyInterval root modus := ⟨0⟩
 /-- Generic interval octave is the same in every key -/
-protected def octave { modus : Hep } : KeyInterval modus := ⟨7⟩
+protected def octave { root modus : Hep } : KeyInterval root modus := ⟨7⟩
 
-instance : ToString (KeyInterval modus) where
+instance : ToString (KeyInterval root modus) where
   toString i :=
     if i.name % 7 == 0 then
       s!"{i.name / 7}"
@@ -306,7 +311,7 @@ instance diatonic (root : Tone) (modus : Hep) : Scale Pitch Interval where
   name := s!"{root} {modus.modus}"
   fundamental := Interval.octave
   pitches := List.finRange 7 |>.map λ i =>
-    let name := i.add root.name
+    let name := i.toNat + root.name.toNat
     -- Nominal shift if the letters are read directly with the same accidentals
     let shiftNominal := (root.name : Fin 7).toNat.repeat List.rotateLeft spaces
       |>.take i.toNat |>.sum
@@ -327,6 +332,7 @@ example : (Pitch.new .c 4) + Interval.octave = (Pitch.new .c 5) := rfl
 example : (Pitch.new .c 4) + Interval.p5 = (Pitch.new .g 4) := rfl
 example : (Pitch.new .b 5) + Interval.p5 = (Pitch.new .f 6 .sharp) := rfl
 example : (Pitch.new .e 3) - (Pitch.new .c 3) = Interval.ma3 := rfl
+example : (diatonic ⟨.d, .natural⟩ .a).pitches = [.new .d 0, .new .e 0, .new .f 0, .new .g 0, .new .a 0, .new .b 0 .flat, .new .c 1] := rfl
 
 abbrev Note := @Prismriver.Note Pitch Rat
 
